src/checker/Pulse.Elaborate.Core.fst
@@ -69,8 +69,8 @@ let elab_bind #g #x #c1 #c2 #c
           (comp_u c2)
           t1 t2
           (comp_pre c1)
-          (mk_abs t1 R.Q_Explicit (comp_post c1))
-          (mk_abs t2 R.Q_Explicit (comp_post c2))
+          (mk_abs0 t1 (comp_post c1))
+          (mk_abs0 t2 (comp_post c2))
           e1 e2
     | C_STGhost inames _ ->
         mk_bind_ghost
@@ -79,8 +79,8 @@ let elab_bind #g #x #c1 #c2 #c
           t1 t2
           inames
           (comp_pre c1)
-          (mk_abs t1 R.Q_Explicit (comp_post c1))
-          (mk_abs t2 R.Q_Explicit (comp_post c2))
+          (mk_abs0 t1 (comp_post c1))
+          (mk_abs0 t2 (comp_post c2))
           e1 e2
     | C_STAtomic inames obs1 _ ->
       let C_STAtomic _ obs2 _ = c2 in      
@@ -92,8 +92,8 @@ let elab_bind #g #x #c1 #c2 #c
           (comp_inames c1)
           t1 t2
           (comp_pre c1)
-          (mk_abs t1 R.Q_Explicit (comp_post c1))
-          (mk_abs t2 R.Q_Explicit (comp_post c2))
+          (mk_abs0 t1 (comp_post c1))
+          (mk_abs0 t2 (comp_post c2))
           e1 e2
   
 let elab_lift #g #c1 #c2 (d:lift_comp g c1 c2) (e:R.term)
@@ -105,7 +105,7 @@ let elab_lift #g #c1 #c2 (d:lift_comp g c1 c2) (e:R.term)
         (comp_u c1)
         (comp_res c1)
         t
-        (mk_abs t R.Q_Explicit (comp_post c1))
+        (mk_abs0 t (comp_post c1))
         e
 
     | Lift_Observability _ c o2 ->
@@ -117,7 +117,7 @@ let elab_lift #g #c1 #c2 (d:lift_comp g c1 c2) (e:R.term)
         (comp_inames c1)
         t
         (comp_pre c1)
-        (mk_abs t R.Q_Explicit (comp_post c1))
+        (mk_abs0 t (comp_post c1))
         e
             
     | Lift_Ghost_Neutral _ _ (| reveal_a, reveal_a_typing |) ->
@@ -126,7 +126,7 @@ let elab_lift #g #c1 #c2 (d:lift_comp g c1 c2) (e:R.term)
         (comp_u c1)
         t
         (comp_pre c1)
-        (mk_abs t R.Q_Explicit (comp_post c1))
+        (mk_abs0 t (comp_post c1))
         e
         reveal_a
 
@@ -136,7 +136,7 @@ let elab_lift #g #c1 #c2 (d:lift_comp g c1 c2) (e:R.term)
         (comp_u c1)
         t
         (comp_pre c1)
-        (mk_abs t R.Q_Explicit (comp_post c1))
+        (mk_abs0 t (comp_post c1))
         e
 
 let intro_pure_tm (p:term) =
@@ -146,9 +146,9 @@ let intro_pure_tm (p:term) =
        (Tm_STApp
         { head =
             tm_pureapp (tm_fvar (as_fv (mk_pulse_lib_core_lid "intro_pure")))
-                       None
+                       R.Q_Explicit
                        p;
-          arg_qual = None;
+          arg_qual = R.Q_Explicit;
           arg = S.wr (`()) rng })
 
 let simple_arr (t1 t2 : R.term) : R.term =
@@ -171,20 +171,16 @@ let rec elab_st_typing (#g:env)
                        (d:st_typing g t c)
   : Tot R.term (decreases d)
   = match d with
-    | T_Abs _ x qual b _u body _c ty_typing body_typing ->
-      let ty = b.binder_ty in
-      let ppname = b.binder_ppname.name in
+    | T_Abs _ x b _u body _c ty_typing body_typing ->
       let body = elab_st_typing body_typing in
-      let b = R.pack_binder { ppname; sort = ty; qual; attrs = [] } in
       mk_abs b (RT.close_term body x) //this closure should be provably redundant by strengthening the conditions on x
 
-
-    | T_STApp _ head _ qual _ arg _ _
-    | T_STGhostApp _ head _ qual _ arg _ _ _ _ ->
-      R.mk_app head [(arg, elab_qual qual)]
+    | T_STApp _ head b _ arg _ _
+    | T_STGhostApp _ head b _ arg _ _ _ _ ->
+      R.mk_app head [(arg, aqualv_for_app (binder_qual b))]
 
     | T_Return _ c use_eq u ty t post _ _ _ _ ->
-      let rp = mk_abs ty R.Q_Explicit post in
+      let rp = mk_abs0 ty post in
       (match c, use_eq with
        | STT, true -> mk_stt_return u ty t rp
        | STT, false -> mk_stt_return_noeq u ty t rp
@@ -197,7 +193,7 @@ let rec elab_st_typing (#g:env)
       let e1 = elab_st_typing e1_typing in
       let e2 = elab_st_typing e2_typing in
       let ty1 = comp_res c1 in
-      elab_bind bc e1 (mk_abs_with_name b.binder_ppname.name ty1 R.Q_Explicit (RT.close_term e2 x))
+      elab_bind bc e1 (mk_abs b (RT.close_term e2 x))
 
     | T_BindFn _ _ _ c1 c2 b x e1_typing _u t_typing e2_typing c2_typing ->
       let e1 = elab_st_typing e1_typing in
@@ -238,23 +234,23 @@ let rec elab_st_typing (#g:env)
     | T_IntroPure _ p _ _ ->
       let head = 
         tm_pureapp (tm_fvar (as_fv (mk_pulse_lib_core_lid "intro_pure")))
-                       None
+                       R.Q_Explicit
                        p
       in
       let arg = (`()) in
-      R.mk_app head [(arg, elab_qual None)]
+      R.mk_app head [(arg, R.Q_Explicit)]
 
     | T_ElimExists _ u t p _ d_t d_exists ->
-      mk_elim_exists u t (mk_abs t R.Q_Explicit p)
+      mk_elim_exists u t (mk_abs0 t p)
 
     | T_IntroExists _ u b p e _ _ _ ->
-      let rt = b.binder_ty in
-      mk_intro_exists u rt (mk_abs rt R.Q_Explicit p) e
+      let rt = binder_sort b in
+      mk_intro_exists u rt (mk_abs0 rt p) e
 
     | T_While _ inv _ _ _ cond_typing body_typing ->
       let cond = elab_st_typing cond_typing in
       let body = elab_st_typing body_typing in
-      mk_while (mk_abs bool_tm R.Q_Explicit inv) cond body
+      mk_while (mk_abs0 bool_tm inv) cond body
 
     | T_Par _ eL cL eR cR _ _ _ eL_typing eR_typing ->
       let ru = comp_u cL in
@@ -270,9 +266,9 @@ let rec elab_st_typing (#g:env)
         raL
         raR
         rpreL
-        (mk_abs raL R.Q_Explicit rpostL)
+        (mk_abs0 raL rpostL)
         rpreR
-        (mk_abs raR R.Q_Explicit rpostR)
+        (mk_abs0 raR rpostR)
         reL reR
 
 		| T_Rewrite _ p q _ _ ->
@@ -282,25 +278,25 @@ let rec elab_st_typing (#g:env)
       let rret_u = comp_u c in
       let rret_t = comp_res c in
       let rpre = comp_pre c in
-      let rpost = mk_abs rret_t R.Q_Explicit (comp_post c) in
+      let rpost = mk_abs0 rret_t (comp_post c) in
       let rbody = elab_st_typing body_typing in
       let rbody = RT.close_term rbody x in
-      let rbody = mk_abs (mk_ref init_t) R.Q_Explicit rbody in
+      let rbody = mk_abs0 (mk_ref init_t) rbody in
       mk_withlocal rret_u init_t init rpre rret_t rpost rbody
 
     | T_WithLocalArray _ _ init len _ init_t c x _ _ _ _ body_typing ->
       let rret_u = comp_u c in
       let rret_t = comp_res c in
       let rpre = comp_pre c in
-      let rpost = mk_abs rret_t R.Q_Explicit (comp_post c) in
+      let rpost = mk_abs0 rret_t (comp_post c) in
       let rbody = elab_st_typing body_typing in
       let rbody = RT.close_term rbody x in
-      let rbody = mk_abs (mk_array init_t) R.Q_Explicit rbody in
+      let rbody = mk_abs0 (mk_array init_t) rbody in
       mk_withlocalarray rret_u init_t init len rpre rret_t rpost rbody
 
     | T_Admit _ c _ ->
       let {u; res; pre; post} = st_comp_of_comp c in
-      let rpost = mk_abs res R.Q_Explicit post in
+      let rpost = mk_abs0 res post in
       (match c with
        | C_ST _ -> mk_stt_admit u res pre rpost
        | C_STAtomic _ _ _ -> mk_stt_atomic_admit u res pre rpost
